WIP

src/specs/PointAddAssign.ec
@@ -4,6 +4,7 @@ require import Array.
 require import EllipticCurve.
 require import Logic.
 require import Memory.
+require import PointAddIntoDest.
 require import PurePrimops.
 require import Real.
 require import RevertWithMessage.
@@ -11,6 +12,11 @@ require import UInt256.
 require import Utils.
 require import YulPrimops.
 require import Verifier.
+
+import MemoryMap.
+
+op to_point (p: int*int): (F*F) = (ZModField.inzmod p.`1, ZModField.inzmod p.`2).
+op from_point (p: F*F): int*int = (ZModField.asint p.`1, ZModField.asint p.`2).
 
 module PointAddAssign = {
   proc low(p1, p2) = {
@@ -30,6 +36,14 @@ module PointAddAssign = {
       RevertWithMessage.low(W256.of_int 28, (W256.of_int STRING (*pointAddAssign: ecAdd failed*)));
     }
   }
+
+  proc mid(p1: int*int, p2: int*int): (int*int) option = {
+    var p1_F, p2_F, result;
+    p1_F <- to_point p1;
+    p2_F <- to_point p2;
+    result <- ecAdd_precompile p1_F.`1 p1_F.`2 p2_F.`1 p2_F.`2;
+    return (omap from_point result);
+  }
 }.
 
 lemma pointAddAssign_extracted_equiv_low :
@@ -45,4 +59,102 @@ proof.
   seq 1 1: (#pre /\ tmp77{1} = _14{2}).
   inline*. wp. skip. by progress.
   inline*. wp. skip. by progress.
-qed. 
+qed.
+
+lemma pointAddAssign_equiv_into_dest :
+equiv [
+    PointAddAssign.low ~ PointAddIntoDest.low:
+      arg{2} = (arg{1}.`1, arg{1}.`2, arg{1}.`1) /\
+      ={glob PointAddAssign} ==>
+      ={glob PointAddAssign}
+    ].
+    proof.
+      proc.
+      seq 9 9: (={glob PointAddAssign} /\ ={_13}).
+      inline Primops.mload Primops.mstore Primops.gas. sp. skip. by progress.
+      seq 1 1: (={glob PointAddAssign} /\ ={_14}).
+      inline*. wp. skip. progress.
+      
+    
+
+import ConcretePrimops.
+
+op pointAddAssign_memory_footprint (mem_0: mem) (p1_address p2_address) =
+  let p1_x = load mem_0 p1_address in
+  let p1_y = load mem_0 (p1_address + W256.of_int 32) in
+  let p2_x = load mem_0 p2_address in
+  let p2_y = load mem_0 (p2_address + W256.of_int 32) in
+  let mem_1 = store mem_0 W256.zero (ecAdd_precompile_unsafe_cast (p1_x, p1_y) (p2_x, p2_y)).`1 in
+  let mem_2 = store mem_1 (W256.of_int 32) (ecAdd_precompile_unsafe_cast (p1_x, p1_y) (p2_x, p2_y)).`2 in
+  let mem_3 = store mem_2 (W256.of_int 64) p2_x in
+  store mem_3 (W256.of_int 96) p2_y.
+
+pred low_inputs_valid (p1_address p2_address: uint256) =
+    W256.of_int 128 <= p1_address /\ W256.of_int 128 <= -p1_address /\
+    W256.of_int 128 <= p2_address /\ W256.of_int 128 <= -p2_address.
+pred mid_inputs_valid (p1 p2: (int*int)) =
+    0 <= p1.`1 < p /\ 0 <= p1.`2 < p /\ 0 <= p2.`1 < p /\ 0 <= p2.`2 < p.
+pred mid_inputs_in_memory (memory: mem) (p1_address p2_address: uint256) (p1 p2: (int*int)) =
+    W256.to_uint (load memory p1_address) = p1.`1 /\
+    W256.to_uint (load memory (p1_address + W256.of_int 32)) = p1.`2 /\
+    W256.to_uint (load memory p2_address) = p2.`1 /\
+    W256.to_uint (load memory (p2_address + W256.of_int 32)) = p2.`2.
+
+lemma pointAddAssign_low_equiv_mid (memory: mem) (p1_address p2_address: uint256) (p1 p2: (int*int)) :
+    equiv [
+      PointAddAssign.low ~ PointAddAssign.mid :
+      low_inputs_valid p1_address p2_address /\
+      mid_inputs_valid p1 p2 /\
+      Primops.memory{1} = memory /\
+      mid_inputs_in_memory memory p1_address p2_address p1 p2 /\
+      arg{1} = (p1_address, p2_address) /\
+      arg{2} = (p1, p2) /\
+      !Primops.reverted{1} ==>
+      (res{2} = None /\ Primops.reverted{1}) \/
+      (
+        exists p, res{2} = Some p /\
+        !Primops.reverted{1} /\
+        Primops.memory{1} = pointAddAssign_memory_footprint memory p1_address p2_address
+      )
+    ].
+    proof.
+      proc.
+      (* Initial memory setup before static_call *)
+      pose mem_1 := store memory W256.zero (load memory p1_address).
+      pose mem_2 := store mem_1 (W256.of_int 32) (load memory (p1_address + W256.of_int 32)).
+      pose mem_3 := store mem_2 (W256.of_int 64) (load memory p2_address).
+      pose mem_4 := store mem_3 (W256.of_int 96) (load memory (p2_address + W256.of_int 32)).
+      seq 8 0 : (
+        low_inputs_valid p1_address p2_address /\
+        mid_inputs_valid p1 p2 /\
+        Primops.memory{1} = mem_4 /\
+        !Primops.reverted{1}
+      ).
+      inline Primops.mload.
+      call{1} (mstore_pspec mem_3 (W256.of_int 96) (load memory (p2_address + W256.of_int 32))). wp. 
+      call{1} (mstore_pspec mem_2 (W256.of_int 64) (load memory p2_address)). wp.
+      call{1} (mstore_pspec mem_1 (W256.of_int 32) (load memory (p1_address + W256.of_int 32))). wp. 
+      call{1} (mstore_pspec memory W256.zero (load memory p1_address)). wp.
+      skip. rewrite /low_inputs_valid. progress.
+      rewrite load_store_diff; [smt (@W256 @Utils) | smt (@W256 @Utils) | reflexivity].
+      rewrite load_store_diff. smt (@W256 @Utils). smt (@W256 @Utils).
+      rewrite /mem_1. rewrite load_store_diff. smt (@W256 @Utils). smt (@W256 @Utils). reflexivity.
+      rewrite load_store_diff. rewrite uint256_le_of_le. simplify. rewrite - addrA.
+      have H_offset: ((W256.of_int 32) - (W256.of_int 64)) = - W256.of_int 32 by smt.
+      rewrite H_offset. rewrite uint256_cast_sub. rewrite W256.of_uintK W256.of_uintK.
+          rewrite pmod_small. rewrite pmod_small. rewrite pmod_small. smt (@W256).
+          progress. smt (@W256 @Utils). smt.
+          progress. smt (@W256 @Utils). smt.
+      rewrite pmod_small. progress. smt (@W256 @Utils). smt. smt (pmod_small @W256 @Utils).
+
+      
+
+
+
+
+
+
+
+
+
+      
